Set_Graphs/Directed_Graphs/Pair_Graph_Specs.thy
@@ -143,8 +143,6 @@ lemma graph_inv_empty: "graph_inv \<emptyset>\<^sub>G"
 definition neighbourhood::"'adjmap \<Rightarrow> 'v \<Rightarrow> 'vset" where
   "(neighbourhood G v) = (case (lookup G v) of Some vset \<Rightarrow> vset | _ \<Rightarrow> vset_empty)"
 
-lemmas [code] = neighbourhood_def
-
 notation "neighbourhood" ("\<N>\<^sub>G _ _" 100)
 
 definition digraph_abs ("[_]\<^sub>g") where "digraph_abs G = {(u,v). v \<in>\<^sub>G (\<N>\<^sub>G G u)}" 
@@ -180,47 +178,8 @@ definition "delete_edge G u v =
     digraph'
   | _ \<Rightarrow> G 
 )"
-(*
-function (domintros) recursive_union where
-"recursive_union us vs = (if us = vset_empty then vs
-                          else let x= sel us in recursive_union (vset_delete x us) (insert x vs))"
-  by pat_completeness auto
 
-partial_function (tailrec) recursive_union_impl where
-"recursive_union_impl us vs = (if us = vset_empty then vs
-                          else let x= sel us in recursive_union_impl (vset_delete x us) (insert x vs))"
-
-lemmas [code] = recursive_union_impl.simps
-
-lemma recursive_union_same:
-  assumes "recursive_union_dom (us, vs)"
-  shows "recursive_union_impl us vs = recursive_union us vs"
-  by(induction rule: recursive_union.pinduct[OF assms])
-    (auto simp add: recursive_union.psimps recursive_union_impl.simps)
-
-lemma recursive_union_finite_dom:
-  assumes "card (t_set us) = n " "finite (t_set us)" "vset_inv us"
-  shows "recursive_union_dom (us, vs)"
-  using assms
-proof(induction n arbitrary: us vs )
-  case 0
-  then show ?case by(auto intro: recursive_union.domintros)
-next
-  case (Suc n)
-  show ?case 
-  apply(rule recursive_union.domintros)
-  using Suc(2-) 
-  by (auto intro:  recursive_union.domintros Suc(1) 
-        simp add: vset.set.set_delete Suc.prems(3) vset.set.invar_delete)
-qed
-
-lemma recursive_union_inv:
-  assumes "recursive_union_dom (us, vs)"  "vset_inv us"  "vset_inv vs"
-  shows "vset_inv ()"
-
-
-definition "union_impl us vs = (if vs = vset_empty then us else recursive_union_impl us vs)"
-*)
+lemmas [code] = neighbourhood_def add_edge_def delete_edge_def
 
 context \<comment>\<open>Locale properties\<close>
   includes vset.set.automation  adjmap.automation
