Spanning_Trees/Encoding.thy
@@ -1,0 +1,183 @@
+theory Encoding
+  imports Directed_Set_Graphs.Pair_Graph_U_Specs Matroids_Greedy.Indep_System_Matroids_Specs
+begin
+
+
+locale Encoding =
+  pair_graph_u: Pair_Graph_U_Specs where lookup = lookup +
+  set2: Set2 where insert = set_insert  and isin = set_isin 
+             and delete = set_delete and invar = set_inv and empty = set_empty
+             and set = to_set
+for lookup :: "'adjmap \<Rightarrow> ('v::linorder) \<Rightarrow> 'vset option"
+ and set_insert :: "('e::linorder) \<Rightarrow> 's \<Rightarrow> 's"  and set_empty and set_delete 
+and set_isin and set_inv and to_set
+and adjmap_fold :: "'adjmap \<Rightarrow> ('v \<Rightarrow> 'vset \<Rightarrow> 's \<Rightarrow> 's) \<Rightarrow> 's \<Rightarrow> 's" and
+    vset_fold :: "'vset \<Rightarrow> ('v \<Rightarrow> 's \<Rightarrow> 's) \<Rightarrow> 's \<Rightarrow> 's" 
+and set_fold_adjmap :: "'s \<Rightarrow> ('e \<Rightarrow> 'adjmap \<Rightarrow> 'adjmap) \<Rightarrow> 'adjmap \<Rightarrow> 'adjmap" and
+    set_fold_vset :: "'s \<Rightarrow> ('e \<Rightarrow> 'vset \<Rightarrow> 'vset) \<Rightarrow> 'vset \<Rightarrow> 'vset" +
+  fixes v1_of :: "'e \<Rightarrow> 'v" and v2_of :: "'e \<Rightarrow> 'v" 
+ and c :: "('v set) \<Rightarrow> rat" and c' :: "'e \<Rightarrow> rat"
+begin
+
+fun edges_to_graph :: "'s \<Rightarrow> 'adjmap" where
+  "edges_to_graph E =
+    set_fold_adjmap E
+    (\<lambda>e G. pair_graph_u.add_edge (pair_graph_u.add_edge G (v1_of e) (v2_of e)) (v2_of e) (v1_of e))
+    empty"
+
+fun edges_to_vertices :: "'s \<Rightarrow> 'vset" where
+  "edges_to_vertices E = 
+    set_fold_vset E
+    (\<lambda>e N. if isin N (v1_of e)
+           then (if isin N (v2_of e) then N else insert (v2_of e) N)
+           else (if isin N (v2_of e) then insert (v1_of e) N else insert (v1_of e) (insert (v2_of e) N)))
+    vset_empty"
+end
+
+locale Encoding_Proofs =
+Encoding +
+assumes adjmap_fold: "\<And> G S f. adjmap_inv G \<Longrightarrow> \<exists> xs. distinct xs \<and> set xs = dom (lookup G) \<and>
+                                 adjmap_fold G f S = foldr (\<lambda> x acc. f x (the (lookup G x)) acc) xs S "
+and set_fold_adjmap: "\<And> G S f.  set_inv S \<Longrightarrow> \<exists> xs. distinct xs \<and> set xs = to_set S \<and>
+                                 set_fold_adjmap S f G = foldr f xs G"
+and vset_fold: "\<And> V f S. vset_inv V \<Longrightarrow> \<exists> xs. distinct xs \<and> set xs = t_set V \<and>
+                                    vset_fold V f S = foldr f xs S"
+and set_fold_vset: "\<And>V f S. set_inv S \<Longrightarrow> \<exists> xs. distinct xs \<and> set xs = to_set S \<and>
+                                 set_fold_vset S f V = foldr f xs V"
+and finite_v_sets: "pair_graph_u.finite_vsets"
+and v1_never_v2:"\<And> e. v1_of e \<noteq> v2_of e"
+begin
+
+lemma pair_graph_u_invar_empty: "pair_graph_u.pair_graph_u_invar \<emptyset>\<^sub>G" 
+proof-
+  have " pair_graph_u.graph_inv \<emptyset>\<^sub>G"
+    by (simp add: pair_graph_u.pair_graph_specs.adjmap.invar_empty pair_graph_u.pair_graph_specs.adjmap.map_empty pair_graph_u.graph_inv_def)
+  moreover have "pair_graph_u.finite_graph \<emptyset>\<^sub>G"
+    by (simp add: pair_graph_u.pair_graph_specs.adjmap.map_empty pair_graph_u.finite_graph_def)
+  ultimately show ?thesis
+    using finite_v_sets 
+    by (unfold pair_graph_u.pair_graph_u_invar_def )
+       (simp add: pair_graph_u.pair_graph_specs.adjmap.map_empty pair_graph_u.neighbourhood_def 
+        pair_graph_u.pair_graph_specs.vset.set.invar_empty pair_graph_u.pair_graph_specs.vset.set.set_empty pair_graph_u.pair_graph_specs.vset.set.set_isin)
+qed
+
+lemma P_of_ifE: "P (if b then x else y) \<Longrightarrow> (b \<Longrightarrow> P x \<Longrightarrow> Q) \<Longrightarrow> (\<not>b \<Longrightarrow> P y \<Longrightarrow> Q) \<Longrightarrow> Q"
+  by(cases b) auto
+
+lemma edges_invar_imp_graph_invar:
+  assumes "set_inv E" shows "pair_graph_u.pair_graph_u_invar (edges_to_graph E)" (is ?thesis1)
+                        and "\<forall> v y. lookup (edges_to_graph E) v = Some y \<longrightarrow> y \<noteq> vset_empty" (is ?thesis2)
+                        and "\<forall> e \<in> pair_graph_u.digraph_abs (edges_to_graph E).
+ lookup (edges_to_graph E) (fst e) \<noteq> None \<longleftrightarrow>  lookup (edges_to_graph E) (snd e) \<noteq> None" (is ?thesis3)
+proof-
+  define f where "f = (\<lambda>e G. pair_graph_u.add_edge (pair_graph_u.add_edge G (v1_of e) (v2_of e)) (v2_of e) (v1_of e))"
+  obtain xs where xs_prop:"distinct xs" "set xs = to_set E" "set_fold_adjmap E f \<emptyset>\<^sub>G = foldr f xs \<emptyset>\<^sub>G"
+    using set_fold_adjmap[OF assms(1), of f empty]  by(auto simp add: f_def)
+  have inv_after_list:"pair_graph_u.pair_graph_u_invar (foldr f xs \<emptyset>\<^sub>G)" for xs
+    by(induction xs)
+      (auto intro: pair_graph_u.pair_graph_u_invar_add_edge simp add: pair_graph_u_invar_empty v1_never_v2  f_def)  
+  then show ?thesis1
+    by(simp add: edges_to_graph.simps f_def[symmetric]  xs_prop(3)) 
+   show ?thesis2
+    unfolding edges_to_graph.simps f_def[symmetric]  xs_prop(3) 
+    apply(induction xs)
+    apply (simp add: pair_graph_u.pair_graph_specs.adjmap.map_empty)
+    apply(subst foldr.simps, subst o_apply, subst f_def)
+    apply(rule pair_graph_u.pair_graph_u_invar_add_edge_both(2))
+    using inv_after_list  v1_never_v2 
+    by (auto intro:  pair_graph_u.pair_graph_u_invar_add_edge_both(2))
+  
+   show ?thesis3
+    unfolding edges_to_graph.simps f_def[symmetric]  xs_prop(3) xs_prop(2)[symmetric]
+  proof(induction xs)
+    case Nil
+    then show ?case 
+      by (simp add: pair_graph_u.pair_graph_specs.adjmap.map_empty)
+  next
+    case (Cons a xs)
+    show ?case 
+      apply(subst (1) foldr.simps, subst o_apply, subst (1) f_def)
+      apply(subst (1) foldr.simps, subst o_apply, subst (2) f_def)
+      apply(subst (1) foldr.simps, subst o_apply, subst (3) f_def)
+    proof( rule, goal_cases)
+      case (1 e)
+      have a1: "pair_graph_u.graph_inv (foldr f xs \<emptyset>\<^sub>G)"
+        by (simp add: inv_after_list)
+      have "(lookup (foldr f xs \<emptyset>\<^sub>G) x \<noteq> None) = (lookup (foldr f xs \<emptyset>\<^sub>G) y \<noteq> None)" 
+        if assms1: "(x, y)\<in>[foldr f xs \<emptyset>\<^sub>G]\<^sub>g" for x y       
+        using pair_graph_u.pair_graph_specs.are_connected_absI[OF assms1 a1]  pair_graph_u.graph_abs_symmetric[OF inv_after_list assms1]
+              pair_graph_u.pair_graph_specs.vset.emptyD(3) pair_graph_u.pair_graph_specs.adjmap.map_empty pair_graph_u.graph_irreflexive[OF  pair_graph_u_invar_empty]
+        by (cases "lookup (foldr f xs \<emptyset>\<^sub>G) x", all \<open>cases "lookup (foldr f xs \<emptyset>\<^sub>G) y"\<close>)
+            (auto split: option.split simp add:  pair_graph_u.digraph_abs_def pair_graph_u.neighbourhood_def)
+      hence ih_prem1: "\<forall>x\<in>[foldr f xs \<emptyset>\<^sub>G]\<^sub>g.
+       (lookup (foldr f xs \<emptyset>\<^sub>G) (fst x) \<noteq> None) = (lookup (foldr f xs \<emptyset>\<^sub>G) (snd x) \<noteq> None)" 
+        by auto
+      show ?case
+        using ih_prem1
+        by(intro bspec[OF pair_graph_u.pair_graph_u_invar_add_edge_both(3)
+               [simplified pair_graph_u.none_symmetry_def], of _ _ _ "(fst e, snd e)", simplified fst_conv snd_conv]
+             ) (auto simp add: inv_after_list v1_never_v2 "1")
+    qed
+  qed
+qed 
+
+lemma digraph_abs_of_edges_of_to_graph:
+  assumes ys_prop: "set ys = to_set E" "set_fold_adjmap E g \<emptyset>\<^sub>G = foldr g ys \<emptyset>\<^sub>G" and
+                g_def: "g = (\<lambda>e G. pair_graph_u.add_edge (pair_graph_u.add_edge G (v1_of e) (v2_of e)) (v2_of e) (v1_of e))" 
+     shows  "[edges_to_graph E]\<^sub>g = (\<lambda> e. (v1_of e, v2_of e)) ` (to_set E) \<union> (\<lambda> e. (v2_of e, v1_of e)) ` (to_set E)"
+proof-
+  have graph_inv_fold_g:"pair_graph_u.graph_inv (foldr g ys \<emptyset>\<^sub>G)" for ys
+    by(induction ys) 
+     (auto intro: simp add: g_def pair_graph_u.pair_graph_specs.adjmap_inv_insert
+            pair_graph_u.pair_graph_specs.graph_inv_empty)
+  show ?thesis
+    unfolding edges_to_graph.simps g_def[symmetric] ys_prop(2) ys_prop(1)[symmetric]
+  proof(induction ys)
+    case Nil
+    then show ?case by(simp add: pair_graph_u.pair_graph_specs.digraph_abs_empty)
+  next
+    case (Cons a ys)   
+    then show ?case 
+    apply simp
+    apply(subst g_def)
+      apply(subst pair_graph_u.digraph_abs_insert[OF pair_graph_u_invar_empty])
+    apply(rule pair_graph_u.adjmap_inv_insert[OF pair_graph_u_invar_empty])
+    apply(rule graph_inv_fold_g)
+    apply(subst pair_graph_u.digraph_abs_insert[OF pair_graph_u_invar_empty])
+      by(auto intro!: graph_inv_fold_g) 
+  qed
+qed
+
+lemma digraph_abs_of_edges_of_to_graph_general:
+  assumes "set_inv E"
+  shows "[edges_to_graph E]\<^sub>g = (\<lambda> e. (v1_of e, v2_of e)) ` (to_set E) \<union> (\<lambda> e. (v2_of e, v1_of e)) ` (to_set E)"
+proof-
+  have set_inv_G:"set_inv E"
+    using assms  by blast
+  define g where "g = (\<lambda>e G. pair_graph_u.add_edge (pair_graph_u.add_edge G (v1_of e) (v2_of e)) (v2_of e) (v1_of e))"
+   obtain xs where xs_prop:"distinct xs" "set xs = to_set E" 
+       "set_fold_adjmap E g empty = foldr g xs empty"
+      using set_fold_adjmap[OF  set_inv_G, of g empty] by blast 
+  show ?thesis
+  by(rule digraph_abs_of_edges_of_to_graph[OF xs_prop(2,3) g_def])
+qed 
+
+find_theorems edges_to_graph
+
+abbreviation "to_doubltn_set X \<equiv> (\<lambda>e. {v1_of e, v2_of e}) ` to_set X"
+
+lemma dbltn_set_and_ugraph_abs:
+  assumes "set_inv X"
+  shows "to_doubltn_set X = pair_graph_u.ugraph_abs (edges_to_graph X)"
+proof-
+   define g where "g =  (\<lambda>e G. pair_graph_u.add_edge (pair_graph_u.add_edge G (v1_of e) (v2_of e)) (v2_of e) (v1_of e))" 
+  obtain xs where xs_prop:" distinct xs" "set xs = to_set X" "set_fold_adjmap X g \<emptyset>\<^sub>G = foldr g xs \<emptyset>\<^sub>G"
+    using set_fold_adjmap[OF assms(1), of g empty] by auto
+  have X_vs_are:"[edges_to_graph X]\<^sub>g = (\<lambda>e. (v1_of e, v2_of e)) ` to_set X \<union> (\<lambda>e. (v2_of e, v1_of e)) ` to_set X"
+    using  digraph_abs_of_edges_of_to_graph[OF xs_prop(2,3) g_def] by simp
+  show ?thesis
+    by(unfold pair_graph_u.ugraph_and_digraph_abs X_vs_are) auto
+qed
+
+end
+end
