Spanning_Trees/Kruskal_Greedy2.thy
@@ -1,0 +1,1026 @@
+theory Kruskal_Greedy2
+  imports Matroids_Greedy.Best_In_Greedy Spanning_Trees Encoding
+         Graph_Algorithms.DFS_Example Insertion_Sort_Desc "HOL-Library.Product_Lexorder"
+begin
+
+hide_const RBT_Set.insert
+global_interpretation Pair_Graph_U_RBT: Pair_Graph_U_Specs
+  where empty = empty and update = update and delete = delete and
+    lookup = lookup and adjmap_inv = "M.invar" and vset_empty = "\<langle>\<rangle>" and
+    insert = vset_insert and vset_delete = vset_delete and vset_inv = "vset_inv::(('v::linorder) rbt \<Rightarrow> bool)" and
+    isin = isin and t_set = "Tree2.set_tree" and sel = sel
+  defines add_edge =Pair_Graph_U_RBT.add_edge
+    and  delete_edge =Pair_Graph_U_RBT.delete_edge
+  by(simp add: Pair_Graph_U_Specs_def Pair_Graph_Specs_def M.Map_axioms S_C.Set_Choose_axioms)
+
+find_theorems add_edge
+
+text \<open>Instantiations for Greedy\<close>
+
+lemma tree_split_case:
+  "(case t of Leaf \<Rightarrow> True | _ \<Rightarrow> False) = (t = Leaf)"
+  by (fastforce split: tree.splits) 
+
+fun rbt_subseteq :: "('a::linorder) rbt \<Rightarrow> 'a rbt \<Rightarrow> bool" where
+  "rbt_subseteq t1 t2 = (case (RBT.diff t1 t2) of Leaf \<Rightarrow> True | _ \<Rightarrow> False)"
+
+lemma rbt_subseteq_correct:
+  "vset_inv t1 \<Longrightarrow> vset_inv t2 \<Longrightarrow> (rbt_subseteq t1 t2) = (Tree2.set_tree t1 \<subseteq> Tree2.set_tree t2)"
+proof(unfold rbt_subseteq.simps tree.split[of "\<lambda> x. x= (_ \<subseteq> _)" True "\<lambda> _ _ _. False" "RBT.diff t1 t2" ],
+      goal_cases)
+  case 1
+  have is_empty_iff:"RBT.diff t1 t2 = \<langle>\<rangle> \<longleftrightarrow> Tree2.set_tree t1 - Tree2.set_tree t2 = {}"
+    using 1  Tree2.eq_set_tree_empty  RBT.set_tree_diff[of t1 t2, symmetric]
+    by (simp add: vset_inv_def)
+  show ?case 
+    using is_empty_iff by (subst Diff_eq_empty_iff[symmetric])fastforce
+qed
+
+lemma rbt_size_correct:
+  "vset_inv X \<Longrightarrow> size X = card (Tree2.set_tree X)"
+  unfolding set_inorder[symmetric]
+proof(induction X rule: inorder.induct)
+  case 1
+  then show ?case by simp
+next
+  case (2 l a uu r)
+  have inter_empty:"set (Tree2.inorder l) \<inter> Set.insert a (set (Tree2.inorder r)) = {}"
+    using 2(3) bst.simps(2)[simplified Tree2.set_inorder[symmetric]]
+    by (metis (no_types, lifting) Int_emptyI insert_iff not_less_iff_gr_or_eq vset_inv_def)
+  have vset_inv_l: "vset_inv l" 
+    by (metis "2.prems" RBT.inv_Node bst.simps(2) vset_inv_def)
+  have vset_inv_r: "vset_inv r" 
+    by (metis "2.prems" RBT.inv_Node bst.simps(2) vset_inv_def)
+  have a_not_down: "a \<notin> set (Tree2.inorder r)" 
+    using 2(3) bst.simps(2)[simplified Tree2.set_inorder[symmetric]] 
+    by (metis not_less_iff_gr_or_eq vset_inv_def)
+  show ?case 
+   using a_not_down inter_empty 
+   by(auto  simp add: card_Un_disjoint card_insert_if  2(1)[OF vset_inv_l] 2(2)[OF vset_inv_r])
+qed
+
+interpretation Custom_Set_RBT: Custom_Set
+  where empty = "\<langle>\<rangle>" and insert = insert_rbt and delete = delete_rbt and invar = "vset_inv::(('e::linorder) rbt \<Rightarrow> bool)" and
+    isin = isin and set = "Tree2.set_tree" and union = "RBT.union" and inter = "RBT.inter" and diff = "RBT.diff" and
+    subseteq = rbt_subseteq and cardinality = size
+  apply (subst Custom_Set_def)
+  apply(intro conjI)
+  subgoal
+    using RBT.Set2_axioms
+    by (metis RBT_Set.empty_def dfs.set_ops.Set2_axioms)
+  subgoal
+    apply (subst Custom_Set_axioms_def)
+    using rbt_subseteq_correct rbt_size_correct by blast
+  done
+
+
+definition "set_of_sets_isin f a = f a"
+
+lemma set_of_sets_isin_def': "set_of_sets_isin = id"
+  using set_of_sets_isin_def by fastforce
+
+interpretation Matroid_Specs_Inst: Matroid_Specs
+  where set_empty = "\<langle>\<rangle>" and set_insert = insert_rbt and set_delete = delete_rbt and set_inv = "vset_inv::(('e::linorder) rbt \<Rightarrow> bool)" and
+    set_isin = isin and to_set = "Tree2.set_tree" and union = "RBT.union" and inter = "RBT.inter" and diff = "RBT.diff" and
+    subseteq = rbt_subseteq and cardinality = size and
+    set_of_sets_isin = "set_of_sets_isin :: ('e rbt \<Rightarrow> bool) \<Rightarrow> 'e rbt \<Rightarrow> bool"
+  apply (subst Matroid_Specs_def)
+  apply (subst Indep_System_Specs_def)
+  using Custom_Set_RBT.Custom_Set_axioms by blast
+
+fun rbt_set_fold :: "'a rbt \<Rightarrow> ('a \<Rightarrow> 'b \<Rightarrow> 'b) \<Rightarrow> 'b \<Rightarrow> 'b" where
+  "rbt_set_fold Leaf f acc = acc"
+| "rbt_set_fold (Node l (a, _) r) f acc = rbt_set_fold r f (f a (rbt_set_fold l f acc))"
+
+lemma rbt_set_fold_revinorder: "rbt_set_fold T f acc = foldr f (rev (inorder T)) acc"
+ by(induction T f acc rule: rbt_set_fold.induct) auto
+
+fun rbt_map_fold :: "('a \<times> 'd) rbt \<Rightarrow> ('a \<Rightarrow> 'd \<Rightarrow> 'b \<Rightarrow> 'b) \<Rightarrow> 'b \<Rightarrow> 'b" where
+  "rbt_map_fold Leaf f acc = acc"
+| "rbt_map_fold (Node l ((a, d), _) r) f acc = rbt_map_fold r f (f a d (rbt_map_fold l f acc))"
+
+lemma rbt_map_fold_revinorder: "rbt_map_fold T f acc = foldr (\<lambda> (x, y) acc. f x y acc) (rev (inorder T)) acc"
+ by(induction T f acc rule: rbt_map_fold.induct) auto
+
+global_interpretation Kruskal_Graphs_Matroids: Encoding
+  where empty = RBT_Set.empty and update = update and delete = RBT_Map.delete and
+    lookup = lookup and adjmap_inv = "M.invar" and vset_empty = "\<langle>\<rangle>" and
+    insert = insert_rbt and vset_delete = delete_rbt and vset_inv = "vset_inv::(('v::linorder) rbt \<Rightarrow> bool)" and
+    isin = isin and t_set = "Tree2.set_tree" and sel = sel and
+
+    set_empty = "\<langle>\<rangle>" and set_insert = insert_rbt and set_delete = delete_rbt and set_inv = "vset_inv::(('e::linorder) rbt \<Rightarrow> bool)" and
+    set_isin = isin and to_set = "Tree2.set_tree" and union = "RBT.union" and inter = "RBT.inter" and diff = "RBT.diff" and
+    adjmap_fold = "rbt_map_fold" and vset_fold = "rbt_set_fold" and set_fold_adjmap = "rbt_set_fold" and
+    set_fold_vset = "rbt_set_fold"
+    for v1_of :: "('e::linorder) \<Rightarrow> ('v::linorder)" and v2_of :: "('e::linorder) \<Rightarrow> ('v::linorder)" (*and 
+        edge_of :: "('v::linorder) \<Rightarrow> 'v \<Rightarrow> ('e::linorder)"*) and c :: "('v set) \<Rightarrow> rat" and c' :: "'e \<Rightarrow> rat"
+      defines (*graph_to_edges = Kruskal_Graphs_Matroids.graph_to_edges
+and*) edges_to_graph = Kruskal_Graphs_Matroids.edges_to_graph
+and edges_to_vertices = Kruskal_Graphs_Matroids.edges_to_vertices
+  by (auto intro: Encoding.intro simp add: Custom_Set_RBT.Set2_axioms Pair_Graph_U_RBT.Pair_Graph_U_Specs_axioms)
+
+
+
+lemma map_of_dom_is:"set (map fst list) = {a. AList_Upd_Del.map_of list a \<noteq> None}"
+proof(induction list)
+  case Nil
+  then show ?case by simp
+next
+  case (Cons a list)
+  have "set (map fst (a # list)) = Set.insert (fst a) (set (map fst list))" by simp
+  also have "... = Set.insert (fst a) {a. AList_Upd_Del.map_of list a \<noteq> None}" 
+    using Cons by simp
+  also have "... =  {aa. AList_Upd_Del.map_of (a # list) aa \<noteq> None}"
+    by(cases a) auto
+  finally show ?case by simp
+qed
+
+lemma map_of_rev: "distinct (map fst xs) \<Longrightarrow> map_of (rev xs) x = map_of xs x"
+  by(induction xs)
+    (auto simp add: map_of_append map_of_dom_is[simplified] split: option.split)
+
+lemma  rbt_map_fold_correct: "M.invar G \<Longrightarrow>
+       \<exists>xs. distinct xs \<and>
+            set xs = dom (lookup G) \<and> rbt_map_fold G f S = foldr (\<lambda>x. f x (the (lookup G x))) xs S"
+proof(subst rbt_map_fold_revinorder, rule exI[of _ "map fst (rev (inorder G))"], goal_cases)
+  case 1
+  have invar_inorder:"rbt G \<and> sorted1 (Tree2.inorder G)"
+   using "1" M.invar_def by auto
+  define list where "list = Tree2.inorder G"
+  define list' where "list' = rev (inorder G)"
+  have distinct_list:"distinct (map fst (Tree2.inorder G))" 
+    using "1" M.invar_def strict_sorted_iff by blast
+  moreover have "set (map fst (Tree2.inorder G)) = dom (lookup G)"
+    using invar_inorder
+    by(subst dom_def, subst M.inorder_lookup, unfold list_def[symmetric] map_of_dom_is) simp+
+  moreover have "foldr (\<lambda>(x, y). f x y) (rev (Tree2.inorder G)) S =
+    foldr (\<lambda>x. f x (the (lookup G x))) (map fst (rev (Tree2.inorder G))) S"
+  proof-
+    have "distinct (map fst list')" 
+      by (metis distinct_list distinct_rev list'_def rev_map)
+    hence same_fold:"foldr (\<lambda>(x, y). f x y) list' S =
+    foldr (\<lambda>x. f x (the (AList_Upd_Del.map_of list' x))) (map fst list') S"
+    proof(induction list')
+      case Nil
+      then show ?case by simp
+    next
+      case (Cons a list')
+      show ?case 
+      proof(cases a)
+        case (Pair x y)
+        have distinct_fsts: "distinct (x # map fst list')" 
+          using Cons(2)[simplified Pair list.map(2) fst_conv] by fast
+        have first_f_apply:"foldr (\<lambda>a. case a of (x, y) \<Rightarrow> f x y) (a # list') S = f x y (foldr (\<lambda>(x, y). f x y) list' S)"
+          by(simp add: Pair)
+        have map_of_same:"(foldr (\<lambda>xa. f xa (the (AList_Upd_Del.map_of ((x, y) # list') xa))) (map fst list') S)
+              = (foldr (\<lambda>xa. f xa (the (AList_Upd_Del.map_of  list' xa))) (map fst list') S)"
+          apply(rule foldr_cong[OF refl refl])
+          subgoal for s t
+            using distinct_fsts[simplified distinct.simps(2)] 
+            by (subst map_of.simps, subst if_not_P)force+
+          done
+        have almost_result: "(foldr (\<lambda>(x, y). f x y) list' S) =
+                   (foldr (\<lambda>xa. f xa (the (AList_Upd_Del.map_of ((x, y) # list') xa))) (map fst list') S)"
+          using distinct_fsts[simplified distinct.simps(2)]
+          by (subst map_of_same, subst Cons(1)[symmetric])force+
+        show ?thesis
+          apply(subst  first_f_apply)
+          apply(subst Pair)+
+          apply(subst  list.map(2))
+          apply(subst foldr.simps)
+          apply(subst o_apply)
+          apply(subst map_of.simps)
+          apply(subst if_P)
+          apply simp
+          apply(subst option.sel)
+          apply(subst fst_conv)
+          by(subst almost_result[symmetric] ) force
+      qed
+    qed
+    show ?thesis
+    using invar_inorder 
+    by(simp add:  lookup_map_of map_of_rev[OF distinct_list, symmetric] list'_def[symmetric] same_fold)+  
+  qed
+ ultimately show ?case 
+   by (metis distinct_rev rev_map set_rev)
+qed
+
+lemma bst_distinct_inorder:"bst T \<Longrightarrow> distinct (inorder T)"
+  by(induction T rule: inorder.induct) fastforce+
+
+lemma rbt_set_fold_correct: "vset_inv S \<Longrightarrow> \<exists>xs. distinct xs \<and> set xs = Tree2.set_tree S \<and> rbt_set_fold S f G = foldr f xs G"
+  apply(subst rbt_set_fold_revinorder)
+  apply(rule exI[of _ "rev (Tree2.inorder S)"])
+  using  bst_distinct_inorder[of S]
+  by(unfold set_inorder[symmetric] set_rev distinct_rev)(simp add: vset_inv_def )
+
+locale Transforms =
+fixes v1_of::"('e::linorder \<Rightarrow> 'v::linorder)" and v2_of::"'e \<Rightarrow> 'v" 
+and input_G :: "'e rbt"
+begin
+
+definition Kruskal_E_to_G :: "('e::linorder) rbt \<Rightarrow> ('v \<times> ('v rbt)) rbt" where
+  "Kruskal_E_to_G = edges_to_graph v1_of v2_of"
+
+definition Kruskal_E_to_V :: "('e::linorder) rbt \<Rightarrow> ('v rbt)" where
+  "Kruskal_E_to_V = edges_to_vertices v1_of v2_of"
+
+definition indep_graph_matroid :: "('e::linorder) rbt \<Rightarrow> bool" where
+  "indep_graph_matroid = (\<lambda> E. undirected_multigraph_spec.has_no_cycle_multi (\<lambda> e. {v1_of e, v2_of e})
+                              (Tree2.set_tree input_G) (Tree2.set_tree E))"
+
+definition "local_indep_oracle e X = 
+((rbt_subseteq (vset_insert e X) input_G) \<and>
+                   (lookup (Kruskal_E_to_G X) (v2_of e) \<noteq> None \<and> lookup (Kruskal_E_to_G X) (v1_of e) \<noteq> None\<longrightarrow>
+                   return (dfs_impl (Kruskal_E_to_G X) (v2_of e) (dfs_initial_state (v1_of e))) 
+                    = NotReachable))"
+
+end
+
+global_interpretation transforms: Transforms
+  where v1_of = v1_of and v2_of = v2_of  and input_G = input_G
+  for v1_of::"'e::linorder \<Rightarrow> 'a::linorder" and v2_of edge_of input_G
+  defines Kruskal_E_to_G=transforms.Kruskal_E_to_G
+   and Kruskal_E_to_V=transforms.Kruskal_E_to_V
+   and indep_graph_matroid=transforms.indep_graph_matroid
+   and local_indep_oracle= transforms.local_indep_oracle
+  done
+
+global_interpretation Kruskal_Greedy: Best_In_Greedy'
+  where set_empty = "\<langle>\<rangle>" and set_insert = insert_rbt and set_delete = delete_rbt 
+     and set_inv = "vset_inv::(('e::linorder) rbt \<Rightarrow> bool)" and
+    set_isin = isin and to_set = "Tree2.set_tree" and union = "RBT.union" and inter = "RBT.inter" and diff = "RBT.diff" and
+    subseteq = rbt_subseteq and cardinality = size and
+    set_of_sets_isin = "set_of_sets_isin :: (('e::linorder) rbt \<Rightarrow> bool) \<Rightarrow> 'e rbt \<Rightarrow> bool" and 
+    carrier = input_G and 
+    indep_set = "indep_graph_matroid v1_of v2_of input_G" and
+    sort_desc = insort_key_desc and 
+    local_indep_oracle = "local_indep_oracle v1_of v2_of input_G"
+    and wrapper_insert = insert_rbt
+and wrapper_invar = "vset_inv::(('e::linorder) rbt \<Rightarrow> bool)"
+and remove_wrapper = id
+and wrapper_empty = Leaf
+  for v1_of::"'e::linorder \<Rightarrow>'a::linorder" and v2_of input_G
+  defines kruskal' = Kruskal_Greedy.BestInGreedy'
+    and  kruskal = Kruskal_Greedy.BestInGreedy
+    and   kruskal_init = Kruskal_Greedy.initial_state
+    and   kruskal_init' = Kruskal_Greedy.initial_state'
+    and indep' = "Kruskal_Greedy.indep'"
+    and to_ordinary = Kruskal_Greedy.to_ordinary
+  apply (subst Best_In_Greedy'_def, subst Best_In_Greedy_def)
+ by(auto intro!: Best_In_Greedy'_axioms.intro 
+simp add: Matroid_Specs_Inst.Matroid_Specs_axioms Pair_Graph_RBT.set.Set_axioms
+ dfs.Graph.vset.set.invar_insert set.invar_empty)
+
+locale Kruskal_Proof_Matroid_Edges =
+Transforms where v1_of = "v1_of::'e::linorder \<Rightarrow> 'v::linorder" for v1_of+
+assumes v1_never_v2:"\<And> e. v1_of e \<noteq> v2_of e"
+begin
+
+context 
+  assumes  G_good: "vset_inv input_G"
+begin
+lemma Encoding_Proofs_axioms:
+ " Encoding_Proofs_axioms t_set M.invar vset_inv lookup vset_inv t_set rbt_map_fold
+     rbt_set_fold rbt_set_fold rbt_set_fold v1_of v2_of"(* edge_of"*)
+proof(rule Encoding_Proofs_axioms.intro, goal_cases)
+  case (1 G S f)
+  then show ?case 
+    by (simp add: rbt_map_fold_correct)
+next
+  case (2 G S f)
+  then show ?case 
+    by (simp add: rbt_set_fold_correct)
+next
+  case (3 V f S)
+  then show ?case 
+    by (simp add: rbt_set_fold_correct)
+next
+  case (4 V f S)
+  then show ?case 
+    by (simp add: rbt_set_fold_correct)
+next
+  case 5
+  then show ?case 
+    by (simp add: dfs.Graph.finite_vsetsI)
+next
+  case (6 e)
+  then show ?case 
+    by (simp add: v1_never_v2)
+qed
+(*
+next
+  case (7 x y)
+  then show ?case
+    by (simp add: v1_of_edge_of)
+next
+  case (8 x y)
+  then show ?case
+    by (simp add: v2_of_edge_of)
+qed
+*)
+interpretation Kruskal_Graphs_Matroids_proofs: Encoding_Proofs
+  where empty = RBT_Set.empty and update = update and delete = RBT_Map.delete and
+    lookup = lookup and adjmap_inv = "M.invar" and vset_empty = "\<langle>\<rangle>" and
+    insert = insert_rbt and vset_delete = delete_rbt and vset_inv = "vset_inv::(('v::linorder) rbt \<Rightarrow> bool)" and
+    isin = isin and t_set = "Tree2.set_tree" and sel = sel and
+
+    set_empty = "\<langle>\<rangle>" and set_insert = insert_rbt and set_delete = delete_rbt and set_inv = "vset_inv::(('e::linorder) rbt \<Rightarrow> bool)" and
+    set_isin = isin and to_set = "Tree2.set_tree" and union = "RBT.union" and inter = "RBT.inter" and diff = "RBT.diff" and
+    adjmap_fold = "rbt_map_fold" and vset_fold = "rbt_set_fold" and set_fold_adjmap = "rbt_set_fold" and
+    set_fold_vset = "rbt_set_fold"
+  for c :: "('v set) \<Rightarrow> rat" and c' :: "'e \<Rightarrow> rat"
+  by(auto intro!: Encoding_Proofs.intro  Encoding_Proofs_axioms 
+           simp add: Encoding_def 
+            Pair_Graph_U_RBT.Pair_Graph_U_Specs_axioms Custom_Set_RBT.Set2_axioms)
+
+lemma pair_graph_u_invar:
+"vset_inv S \<Longrightarrow> Pair_Graph_U_RBT.pair_graph_u_invar (Kruskal_E_to_G S)"
+  by (simp add: Kruskal_Graphs_Matroids_proofs.edges_invar_imp_graph_invar edges_to_graph_def local.Kruskal_E_to_G_def)
+
+lemma same_dgraphabs:"dfs.Graph.digraph_abs = G.digraph_abs"
+  by (simp add: RBT_Set.empty_def)
+
+abbreviation "to_dbltn == (\<lambda>x. {v1_of x, v2_of x})"
+
+lemma to_dbltn_sym: "{v2_of x, v1_of x} = to_dbltn x" by auto
+
+interpretation undirected_multigraph: undirected_multigraph to_dbltn "Tree2.set_tree G"
+  using v1_never_v2 by (auto intro!:  undirected_multigraph.intro)
+
+lemma local_indep_oracle_correct:
+  assumes "vset_inv S"
+        "indep' v1_of v2_of input_G (id S)"
+        "rbt_subseteq (id S) input_G"
+        "e \<notin> t_set (id S)"
+ shows "local_indep_oracle e S = indep' v1_of v2_of input_G (vset_insert e (id S))"
+  apply(insert assms)
+  unfolding indep'_def Matroid_Specs_Inst.indep_def Kruskal_Greedy2.indep_graph_matroid_def
+            indep_graph_matroid_def set_of_sets_isin_def 
+proof(goal_cases)
+  case 1
+  note case_assms = this
+  have first_eq:"rbt_subseteq (vset_insert e S) input_G = (t_set (vset_insert e (id S)) \<subseteq> t_set input_G)" 
+    using G_good assms(1) dfs.Graph.vset.set.invar_insert rbt_subseteq_correct by auto
+  have second_eq:"(((lookup (local.Kruskal_E_to_G S) (v2_of e) \<noteq> None \<and> lookup (Kruskal_E_to_G S) (v1_of e) \<noteq> None) \<longrightarrow>
+                 (return (dfs_impl (local.Kruskal_E_to_G S) (v2_of e) 
+                 (dfs_initial_state (v1_of e))) = NotReachable))) =
+                (\<nexists>u. Ex (undirected_multigraph_spec.decycle_multi (\<lambda>e. {v1_of e, v2_of e}) (t_set (vset_insert e (id S)))u))"
+    if additional_assm: "insert e (t_set  S) \<subseteq> t_set input_G"
+  proof-
+    have digraph_abs_is:"G.digraph_abs (Kruskal_E_to_G S) =
+     (\<lambda>e. (v1_of e, v2_of e)) ` t_set S \<union> (\<lambda>e. (v2_of e, v1_of e)) ` t_set S"
+     by(auto intro!: Kruskal_Graphs_Matroids_proofs.digraph_abs_of_edges_of_to_graph_general
+            simp add: assms(1) Kruskal_E_to_G_def edges_to_graph_def )
+   have ugraph_abs_is: "Pair_Graph_U_RBT.ugraph_abs (Kruskal_E_to_G S) = to_dbltn ` (t_set  S)"
+    by(auto intro!: Kruskal_Graphs_Matroids_proofs.dbltn_set_and_ugraph_abs[symmetric]
+            simp add: assms(1) Kruskal_E_to_G_def edges_to_graph_def )
+   have pair_graph_u_invar:"Pair_Graph_U_RBT.pair_graph_u_invar (edges_to_graph  v1_of  v2_of S)" 
+     using assms(1) local.Kruskal_E_to_G_def pair_graph_u_invar by auto
+   have double_ex_I: "rest x y \<Longrightarrow> \<exists>v1 v2.
+       {x, y} = {v1, v2} \<and> rest v1 v2" for x y rest by auto
+   have lookup_in_dVs:"lookup (local.Kruskal_E_to_G S) x = Some y\<Longrightarrow> 
+          x \<in> dVs (dfs.Graph.digraph_abs (local.Kruskal_E_to_G S))" for x y
+     using Kruskal_Graphs_Matroids_proofs.edges_invar_imp_graph_invar(2)[OF assms(1)]
+            S_C.choose  
+     by(unfold  dfs.Graph.digraph_abs_def DFS_Example.neighbourhood_def)
+       (auto simp add: Kruskal_E_to_G_def edges_to_graph_def
+                      neighbourhood_def[symmetric] dfs.Graph.neighbourhood_def dVs_def
+               intro!: exI[of _ "{x, sel y}"]  double_ex_I)
+   have "lookup (local.Kruskal_E_to_G S) (v1_of e) = Some y \<Longrightarrow>
+         DFS.DFS_axioms isin t_set adj_inv vset_empty vset_inv lookup
+          (local.Kruskal_E_to_G S) (v1_of e)" for y
+     unfolding DFS.DFS_axioms_def[OF dfs.DFS_axioms]
+     using   lookup_in_dVs pair_graph_u_invar
+     by(unfold Pair_Graph_U_RBT.pair_graph_u_invar_def Kruskal_E_to_G_def adj_inv_def)
+     simp
+   hence DFS_thms: "lookup (local.Kruskal_E_to_G S) (v1_of e) \<noteq> None \<Longrightarrow>
+        DFS_thms map_empty RBT_Map.delete vset_insert isin t_set sel update adj_inv vset_empty vset_delete vset_inv
+     vset_union vset_inter vset_diff lookup (Kruskal_E_to_G S) (v1_of e)"
+     by(auto intro!: DFS_thms.intro dfs.DFS_axioms DFS_thms_axioms.intro )
+   have graph_abs_with_e: "graph_abs (to_dbltn ` insert e (t_set S))"
+     using v1_never_v2 by (auto simp add: graph_abs_def dblton_graph_def Vs_def)
+   have graph_abs_without_e: "graph_abs (to_dbltn `(t_set S))"
+     using graph_abs_mono graph_abs_with_e by auto
+   have graph_abs_vset_insert:"graph_abs (to_dbltn ` t_set (vset_insert e S))"
+     using RBT.set_tree_insert[of S] case_assms(1) graph_abs_with_e 
+     by(simp add:vset_inv_def)
+   show ?thesis 
+     unfolding dfs_impl_def dfs_initial_state_def
+   proof(cases "lookup (local.Kruskal_E_to_G S) (v1_of e) \<noteq> None 
+         \<and> lookup (local.Kruskal_E_to_G S) (v2_of e) \<noteq> None", goal_cases)
+     case 1
+     hence 1: "lookup (local.Kruskal_E_to_G S) (v1_of e) \<noteq> None" 
+              "lookup (local.Kruskal_E_to_G S) (v2_of e) \<noteq> None" by auto
+     note one = this
+     show ?case
+     proof(subst DFS_thms.DFS_to_DFS_impl[OF DFS_thms, symmetric, OF 1(1)], rule, all \<open>rule ccontr\<close>, goal_cases)
+       case 1
+       then obtain u C where uC_prop:"undirected_multigraph_spec.decycle_multi to_dbltn
+                 (t_set (vset_insert e S)) u C" by auto
+       moreover have  not_cycle_old:"\<not> undirected_multigraph_spec.decycle_multi to_dbltn
+                 (t_set S) u C" 
+         using case_assms(2) 
+         by(simp add: id_def undirected_multigraph_spec.has_no_cycle_multi_def)
+       ultimately have e_and_C:"e \<in> set C" "set C \<subseteq> (t_set (vset_insert e S))"
+         unfolding undirected_multigraph_spec.decycle_multi_def     
+        using epath_subset_other_set[of "insert {v1_of e, v2_of e} (to_dbltn ` t_set S)"
+                                    u "map _ C" u , simplified list.set_map,OF _ image_mono] 
+        by (auto simp add: Pair_Graph_RBT.set.set_insert[OF case_assms(1)])
+      then obtain C1 C2 where C_split:"C = C1@[e]@C2"
+        by (metis append_Cons append_self_conv2 split_list_last)
+      obtain q where q_prop:"walk_betw (to_dbltn ` (insert e (t_set S))) u q u" "map to_dbltn C = edges_of_path q"
+        using graph_abs.epath_imp_walk_betw[of _ u "map to_dbltn C" u, OF graph_abs_with_e] 
+              uC_prop 
+         by(auto simp add: undirected_multigraph_spec.decycle_multi_def  Pair_Graph_RBT.set.set_insert[OF case_assms(1)])
+      
+       hence e_in_p: "to_dbltn e \<in> set (edges_of_path q)"
+        by (metis (mono_tags, lifting) \<open>e \<in> set C\<close> image_set rev_image_eqI)
+      have lengthq: "length q \<ge> 2" 
+        using \<open>to_dbltn e \<in> set (edges_of_path q)\<close> edges_of_path_nempty by fastforce
+      have v1v2: "v1_of e \<noteq> v2_of e" 
+        by (simp add: v1_never_v2)
+    show ?case proof(cases "lookup (local.Kruskal_E_to_G S) (v2_of e)")
+      case None
+       thus ?thesis 
+        by (simp add: one(2))
+    next
+      case (Some neighb)
+      have "\<exists>q. walk_betw (to_dbltn ` t_set (vset_insert e S)) u q u \<and> map to_dbltn C = edges_of_path q"
+        using graph_abs_vset_insert  uC_prop 
+        by(auto intro:graph_abs.epath_imp_walk_betw simp add: undirected_multigraph.decycle_multi_def)
+      have no_distinct_path:"\<nexists>p. distinct p \<and>
+              vwalk_bet (dfs.Graph.digraph_abs (local.Kruskal_E_to_G S)) (v1_of e) p (v2_of e)"
+        using DFS_thms.DFS_correct_1[OF DFS_thms] Some  one 1 by blast
+      have no_other_e:"(to_dbltn e) \<notin> (to_dbltn ` t_set S)"
+      proof(rule, rule ccontr, goal_cases)
+        case 1
+        then obtain d where d_prop:"to_dbltn d = to_dbltn e" "d \<in> t_set S" by auto
+        hence "{(v1_of d, v2_of d), (v2_of d, v1_of d)} \<subseteq> (dfs.Graph.digraph_abs (local.Kruskal_E_to_G S))"
+          by (simp add: RBT_Set.empty_def digraph_abs_is)
+        moreover have "(v1_of e, v2_of e) = (v1_of d, v2_of d)\<or>(v1_of e, v2_of e) = (v2_of d, v1_of d)"
+          using d_prop by(unfold doubleton_eq_iff) presburger
+        ultimately have "vwalk_bet (dfs.Graph.digraph_abs (Kruskal_E_to_G S)) 
+                         (v1_of e) [v1_of e, v2_of e] (v2_of e)" 
+          by fastforce
+        moreover have "distinct [v1_of e, v2_of e]"
+          using v1v2 by auto
+        ultimately show ?case 
+          using   no_distinct_path by blast
+      qed 
+      moreover have dbltn_inj:"inj_on to_dbltn (t_set S) "
+        using case_assms(2) undirected_multigraph.has_no_cycle_multi_to_dbltn_inj by simp
+      ultimately have dbltn_inj_big:"inj_on to_dbltn (insert e (t_set S))" by auto
+      moreover have C_subset:"set C \<subseteq> (insert e (t_set S))"
+        using case_assms(1) dfs.Graph.vset.set.set_insert e_and_C(2) by auto
+      ultimately have inj_C:"inj_on to_dbltn (set C)" 
+        by (meson inj_on_subset)
+      have distinct_edges_q:"distinct (edges_of_path q)"
+        using q_prop(2) distinct_map[of to_dbltn C] uC_prop e_and_C inj_C
+        by(auto simp add: undirected_multigraph.decycle_multi_def) 
+      have e_vs_in_new_v_set:"{v1_of e, v2_of e} \<subseteq> Vs (to_dbltn ` insert e (t_set S))"
+        by (simp add: vs_member)
+      then obtain q1 q2 where q1_q2_prop: "q = q1@[v1_of e, v2_of e]@ q2 \<or> q = q1@[v2_of e, v1_of e]@ q2"
+        using undirected_multigraph.edges_to_path_split_by_edge[of _ _ "v1_of e" "v2_of e"] e_in_p by fast
+       obtain q' where  path_without_e:"walk_betw (to_dbltn `  (t_set S)) (v1_of e) q' (v2_of e)"
+       proof(cases rule: disjE[OF q1_q2_prop], all "cases q1", all \<open>cases q2\<close>, goal_cases)
+         case 1
+         then show ?case 
+           using q_prop(1) v1v2 walk_between_nonempty_pathD(3) walk_between_nonempty_pathD(4) by fastforce
+       next
+         case (2 a list)
+         hence a1:"walk_betw (to_dbltn ` insert e (t_set S)) u (q1 @ [v1_of e]) (v1_of e)"
+           using q_prop(1) by (intro walk_pref[of _ u q1 "v1_of e" "v2_of e # q2" u]) force
+         moreover have a2:"walk_betw (to_dbltn ` insert e (t_set S)) (v2_of e) (v2_of e # q2) u"
+           using q_prop(1) 2(2)  by(intro walk_suff[of _ u "q1@[v1_of e]" "v2_of e" q2 u]) force 
+         ultimately have a3:"walk_betw (to_dbltn ` insert e (t_set S)) (v2_of e) ([v2_of e] @ q2) (v1_of e)"
+           by (simp add: "2"(3) walk_betw_def)
+         have a4:"set (edges_of_path ([v2_of e] @ q2)) \<subseteq> set (edges_of_path q)"
+           using "2"(2) "2"(3) by auto
+         moreover have a5:"to_dbltn e \<notin> set (edges_of_path ([v2_of e] @ q2))" 
+           using "2"(2) "2"(3) distinct_edges_q by auto
+         ultimately have a6:"set (edges_of_path ([v2_of e] @ q2)) \<subseteq> (to_dbltn `(t_set S))" 
+           using a3 graph_abs.path_ball_edges' graph_abs_with_e walk_between_nonempty_pathD(1) by fastforce
+         have "walk_betw (to_dbltn `(t_set S)) (v2_of e) ([v2_of e] @ q2) (v1_of e)"  
+           using walk_betw_strengthen[OF a3 _ a6] 2(4) by simp
+         hence "walk_betw (to_dbltn `(t_set S)) (v1_of e) (rev ([v2_of e] @ q2)) (v2_of e)" 
+           by (meson walk_symmetric)
+         thus ?case
+           using 2(1) by simp         
+       next
+         case (3 a list)
+         hence a1:"walk_betw (to_dbltn ` insert e (t_set S)) u (q1 @ [v1_of e]) (v1_of e)"
+           using q_prop(1) by (intro walk_pref[of _ u q1 "v1_of e" "v2_of e # q2" u]) force
+         moreover have a2:"walk_betw (to_dbltn ` insert e (t_set S)) (v2_of e) (v2_of e # q2) u"
+           using q_prop(1) 3(2)  by(intro walk_suff[of _ u "q1@[v1_of e]" "v2_of e" q2 u]) force 
+         ultimately have a3:"walk_betw (to_dbltn ` insert e (t_set S)) (v2_of e) (q1@ [v1_of e] ) (v1_of e)"
+           by (simp add: "3"(4) walk_betw_def)
+         have a4:"set (edges_of_path (q1@ [v1_of e])) \<subseteq> set (edges_of_path q)" 
+           using 3(2-) edges_of_path_append_subset_2 by fastforce
+         moreover have a5:"to_dbltn e \<notin> set (edges_of_path (q1@ [v1_of e]))" 
+           using  distinct_edges_q by(unfold 3(2) edges_of_path_symmetric_split) simp
+         ultimately have a6:"set (edges_of_path (q1@ [v1_of e])) \<subseteq> (to_dbltn `(t_set S))" 
+           using a3 graph_abs.path_ball_edges' graph_abs_with_e walk_between_nonempty_pathD(1) by fastforce
+         have "walk_betw (to_dbltn `(t_set S)) (v2_of e) (q1@ [v1_of e]) (v1_of e)"  
+           using walk_betw_strengthen[OF a3 _ a6] 3(3) by simp
+         hence "walk_betw (to_dbltn `(t_set S)) (v1_of e) (rev (q1@ [v1_of e])) (v2_of e)" 
+           by (meson walk_symmetric)
+         thus ?case
+           using 3(1) by simp 
+       next
+         case (4 a list aa lista)
+         hence a1:"walk_betw (to_dbltn ` insert e (t_set S)) u (q1 @ [v1_of e]) (v1_of e)"
+           using q_prop(1) by (intro walk_pref[of _ u q1 "v1_of e" "v2_of e # q2" u]) force
+         moreover have a2:"walk_betw (to_dbltn ` insert e (t_set S)) (v2_of e) (v2_of e # q2) u"
+           using q_prop(1) 4(2)  by(intro walk_suff[of _ u "q1@[v1_of e]" "v2_of e" q2 u]) force     
+         have a4:"set (edges_of_path (q1@ [v1_of e])) \<subseteq> set (edges_of_path q)" 
+           using 4(2-) edges_of_path_append_subset_2 by fastforce
+         moreover have a5:"to_dbltn e \<notin> set (edges_of_path (q1@ [v1_of e]))" 
+           using  distinct_edges_q by(unfold 4(2) edges_of_path_symmetric_split) simp
+         ultimately have a6:"set (edges_of_path (q1@ [v1_of e])) \<subseteq> (to_dbltn `(t_set S))" 
+           using graph_abs.path_ball_edges' graph_abs_with_e walk_between_nonempty_pathD(1) by fastforce
+         have a4:"set (edges_of_path ([v2_of e] @ q2)) \<subseteq> set (edges_of_path q)"
+           using "4"(2) edges_of_path_append_subset by fastforce
+         moreover have a5:"to_dbltn e \<notin> set (edges_of_path ([v2_of e] @ q2))" 
+           using  "4"(4) distinct_edges_q by(unfold 4(2) edges_of_path_symmetric_split) simp 
+         moreover have a3:"walk_betw (to_dbltn ` insert e (t_set S)) (v2_of e) ([v2_of e] @ q2) u"
+           using a2 a1 by simp 
+         ultimately have a7:"set (edges_of_path ([v2_of e] @ q2)) \<subseteq> (to_dbltn `(t_set S))"
+           using  a1 a2 graph_abs.path_ball_edges' graph_abs_with_e walk_between_nonempty_pathD(1) by fast 
+         have "walk_betw (to_dbltn `(t_set S)) u (q1@ [v1_of e]) (v1_of e)"  
+           using walk_betw_strengthen 4(3) a1 a6 by fastforce
+         moreover have "walk_betw (to_dbltn `(t_set S)) (v2_of e) ( [v2_of e]@q2)u"  
+           using walk_betw_strengthen 4(3)  "4"(4) a3 a7 by fastforce
+         ultimately have  "walk_betw (to_dbltn `(t_set S)) (v2_of e) ( ([v2_of e]@q2@(tl q1)@[v1_of e])) (v1_of e)" 
+           using "4"(3) walk_transitive_2 by fastforce
+         then show ?case 
+           using 4(1)[of "rev ([v2_of e]@q2@(tl q1)@[v1_of e])"]
+           by (meson walk_symmetric)
+       next
+         case 5
+         then show ?case 
+           using q_prop(1) v1v2 walk_between_nonempty_pathD(3) walk_between_nonempty_pathD(4) by fastforce
+       next
+         case (6 a list)
+         hence a1:"walk_betw (to_dbltn ` insert e (t_set S)) u (q1 @ [v2_of e]) (v2_of e)"
+           using q_prop(1) by (intro walk_pref[of _ u q1 "v2_of e" "v1_of e # q2" u]) force
+         moreover have a2:"walk_betw (to_dbltn ` insert e (t_set S)) (v1_of e) (v1_of e # q2) u"
+           using q_prop(1) 6(2)  by(intro walk_suff[of _ u "q1@[v2_of e]" "v1_of e" q2 u]) force 
+         ultimately have a3:"walk_betw (to_dbltn ` insert e (t_set S)) (v1_of e) ([v1_of e] @ q2) (v2_of e)"
+           by (simp add: "6"(3) walk_betw_def)
+         have a4:"set (edges_of_path ([v1_of e] @ q2)) \<subseteq> set (edges_of_path q)"
+           using "6"(2) "6"(3) by auto
+         moreover have a5:"to_dbltn e \<notin> set (edges_of_path ([v1_of e] @ q2))" 
+           using "6"(2) "6"(3) distinct_edges_q 
+           by (simp add: insert_commute)
+         ultimately have a6:"set (edges_of_path ([v1_of e] @ q2)) \<subseteq> (to_dbltn `(t_set S))" 
+           using a3 graph_abs.path_ball_edges' graph_abs_with_e walk_between_nonempty_pathD(1) by fastforce
+         have "walk_betw (to_dbltn `(t_set S)) (v1_of e) ([v1_of e] @ q2) (v2_of e)"  
+           using walk_betw_strengthen[OF a3 _ a6] 6(4) by simp
+         thus ?case
+           using 6(1) by simp         
+       next
+         case (7 a list)
+         hence a1:"walk_betw (to_dbltn ` insert e (t_set S)) u (q1 @ [v2_of e]) (v2_of e)"
+           using q_prop(1) by (intro walk_pref[of _ u q1 "v2_of e" "v1_of e # q2" u]) force
+         moreover have a2:"walk_betw (to_dbltn ` insert e (t_set S)) (v1_of e) (v1_of e # q2) u"
+           using q_prop(1) 7(2)  by(intro walk_suff[of _ u "q1@[v2_of e]" "v1_of e" q2 u]) force 
+         ultimately have a3:"walk_betw (to_dbltn ` insert e (t_set S)) (v1_of e) (q1@ [v2_of e] ) (v2_of e)"
+           by (simp add: "7"(4) walk_betw_def)
+         have a4:"set (edges_of_path (q1@ [v2_of e])) \<subseteq> set (edges_of_path q)" 
+           using 7(2-) edges_of_path_append_subset_2 by fastforce
+         moreover have a5:"to_dbltn e \<notin> set (edges_of_path (q1@ [v2_of e]))" 
+           using  distinct_edges_q by(unfold 7(2) edges_of_path_symmetric_split to_dbltn_sym) auto
+         ultimately have a6:"set (edges_of_path (q1@ [v2_of e])) \<subseteq> (to_dbltn `(t_set S))" 
+           using a3 graph_abs.path_ball_edges' graph_abs_with_e walk_between_nonempty_pathD(1) by fastforce
+         have "walk_betw (to_dbltn `(t_set S)) (v1_of e) (q1@ [v2_of e]) (v2_of e)"  
+           using walk_betw_strengthen[OF a3 _ a6] 7(3) by simp
+         thus ?case
+           using 7(1) by simp 
+       next
+         case (8 a list aa lista)
+         hence a1:"walk_betw (to_dbltn ` insert e (t_set S)) u (q1 @ [v2_of e]) (v2_of e)"
+           using q_prop(1) by (intro walk_pref[of _ u q1 "v2_of e" "v1_of e # q2" u]) force
+         moreover have a2:"walk_betw (to_dbltn ` insert e (t_set S)) (v1_of e) (v1_of e # q2) u"
+           using q_prop(1) 8(2)  by(intro walk_suff[of _ u "q1@[v2_of e]" "v1_of e" q2 u]) force     
+         have a4:"set (edges_of_path (q1@ [v2_of e])) \<subseteq> set (edges_of_path q)" 
+           using 8(2-) edges_of_path_append_subset_2 by fastforce
+         moreover have a5:"to_dbltn e \<notin> set (edges_of_path (q1@ [v2_of e]))" 
+           using  distinct_edges_q by(unfold 8(2) edges_of_path_symmetric_split to_dbltn_sym) simp
+         ultimately have a6:"set (edges_of_path (q1@ [v2_of e])) \<subseteq> (to_dbltn `(t_set S))" 
+           using graph_abs.path_ball_edges' graph_abs_with_e walk_between_nonempty_pathD(1) by fastforce
+         have a4:"set (edges_of_path ([v1_of e] @ q2)) \<subseteq> set (edges_of_path q)"
+           using 8(2) edges_of_path_append_subset by fastforce
+         moreover have a5:"to_dbltn e \<notin> set (edges_of_path ([v1_of e] @ q2))" 
+           using 8(4) distinct_edges_q by(unfold 8(2) edges_of_path_symmetric_split to_dbltn_sym) simp 
+         moreover have a3:"walk_betw (to_dbltn ` insert e (t_set S)) (v1_of e) ([v1_of e] @ q2) u"
+           using a2 a1 by simp 
+         ultimately have a7:"set (edges_of_path ([v1_of e] @ q2)) \<subseteq> (to_dbltn `(t_set S))"
+           using  a1 a2 graph_abs.path_ball_edges' graph_abs_with_e walk_between_nonempty_pathD(1) by fast 
+         have "walk_betw (to_dbltn `(t_set S)) u (q1@ [v2_of e]) (v2_of e)"  
+           using walk_betw_strengthen 8(3) a1 a6 by fastforce
+         moreover have "walk_betw (to_dbltn `(t_set S)) (v1_of e) ( [v1_of e]@q2)u"  
+           using walk_betw_strengthen 8(3)  8(4) a3 a7 by fastforce
+         ultimately have  "walk_betw (to_dbltn `(t_set S)) (v1_of e) ( ([v1_of e]@q2@(tl q1)@[v2_of e])) (v2_of e)" 
+           using 8(3) walk_transitive_2 by fastforce
+         then show ?case using 8(1) by auto
+       qed
+       have  dfs_vwalk:"vwalk_bet (dfs.Graph.digraph_abs (local.Kruskal_E_to_G S)) (v1_of e) q' (v2_of e)"
+         apply(subst same_dgraphabs, subst Pair_Graph_U_RBT.ugraph_abs_digraph_abs[symmetric])
+         using local.Kruskal_E_to_G_def pair_graph_u_invar apply simp
+         using  graph_abs.walk_betw_iff_vwalk_bet[OF graph_abs_without_e]  path_without_e 
+         by (simp  add: ugraph_abs_is )
+       obtain q'' where "vwalk_bet (dfs.Graph.digraph_abs (local.Kruskal_E_to_G S)) (v1_of e) q'' (v2_of e)"
+                             "distinct q''" 
+         using  vwalk_bet_to_distinct_is_distinct_vwalk_bet[OF dfs_vwalk]
+         by(auto simp add: distinct_vwalk_bet_def)
+       thus False 
+         using no_distinct_path by blast
+     qed
+   next
+     case 2
+     note two = this
+     show ?case 
+     proof(cases "lookup (local.Kruskal_E_to_G S) (v2_of e)")
+       case None 
+       hence "lookup (local.Kruskal_E_to_G S) (v1_of e) = None" 
+         using two(2) by blast
+       thus False 
+         by (simp add: one)
+     next
+       case (Some neighbs)
+       hence dfs_reachable:"return
+         (dfs.DFS (local.Kruskal_E_to_G S) (v2_of e) (DFS.initial_state vset_insert vset_empty (v1_of e))) =
+             Reachable" 
+         using two(2) return.exhaust by auto
+       then obtain p where p_vwalk:"vwalk_bet (dfs.Graph.digraph_abs (local.Kruskal_E_to_G S)) (v1_of e)
+                                      p (v2_of e)"
+         using DFS_thms.DFS_correct_2[OF DFS_thms[OF one(1)]] dfs_reachable by auto
+       have walk_betw_around_e:"walk_betw (to_dbltn ` t_set S) (v1_of e) p (v2_of e)"
+         apply(subst  ugraph_abs_is[symmetric], subst graph_abs.walk_betw_iff_vwalk_bet, simp add: graph_abs_without_e ugraph_abs_is)
+         using  pair_graph_u_invar  p_vwalk 
+         by(auto simp add: Pair_Graph_U_RBT.ugraph_abs_digraph_abs same_dgraphabs Kruskal_E_to_G_def)
+       have "epath (to_dbltn ` t_set S) (v1_of e) (edges_of_path p) (v2_of e)" 
+         by(auto intro!: graph_abs.walk_betw_imp_epath simp add: walk_betw_around_e graph_abs_without_e)
+       moreover then obtain p' where p'_prop:"map to_dbltn p' = edges_of_path p" "set p' \<subseteq>  (t_set S)"
+         using undirected_multigraph.edges_of_path_to_multigraph_path[OF epath_edges_subset]
+         by blast 
+       ultimately have epath_first_path:"epath (to_dbltn `  (t_set S)) (v1_of e) (map to_dbltn p') (v2_of e)"  
+         by simp
+       then obtain p'' where p''_prop:"epath (to_dbltn ` t_set S) (v1_of e) p'' (v2_of e)" 
+                       "set p'' \<subseteq> set (map to_dbltn p')" "distinct p''"
+         using  epath_distinct_epath by fast
+       obtain p_mul where p_mul: "map to_dbltn p_mul = p''" "set p_mul \<subseteq> set p'"
+         using p''_prop(2) map_eq_Cons_conv by(induction p'')  fastforce+
+       hence epath_p_mul:"epath (to_dbltn ` t_set S) (v1_of e) (map to_dbltn p_mul) (v2_of e)"
+         using p''_prop(1) by blast
+       hence epath_first_path:"epath (to_dbltn ` (insert e (t_set S))) (v1_of e) (map to_dbltn p_mul) (v2_of e)"  
+         by (auto intro: epath_subset image_mono subset_insertI)
+       moreover have "epath (to_dbltn ` (insert e (t_set S))) (v2_of e) [to_dbltn e] (v1_of e)" 
+         using v1_never_v2[of e] by(auto intro!: epath_single)
+       ultimately have epath3:"epath (to_dbltn ` (insert e (t_set S))) (v1_of e) 
+                              (map to_dbltn (p_mul@[e])) (v1_of e)" 
+         by (auto intro: epath_append)
+       moreover have "set (p_mul@[e]) \<subseteq> insert e (t_set S)" 
+         using p'_prop(2) p_mul(2) by auto
+       moreover have "2 \<le> length (p_mul@[e])" 
+         using epath_non_empty[OF epath_p_mul, simplified length_map] 
+         by (simp add: v1_never_v2)
+       moreover have "distinct (p_mul@[e])" 
+       proof-
+         have "distinct p_mul"
+           using p_mul(1)  p''_prop(3) by (auto simp add: distinct_map)
+         moreover have "set p_mul \<subseteq> t_set S" 
+           using p'_prop(2) p_mul(2) by order
+         ultimately show ?thesis using assms(4) by auto
+       qed
+       ultimately have "undirected_multigraph.decycle_multi (t_set (vset_insert e (id S))) (v1_of e) (p_mul@[e])" 
+          by (simp add: undirected_multigraph.decycle_multi_def  case_assms(1) dfs.Graph.vset.set.set_insert)
+        thus ?thesis 
+         using 2(1) by simp
+     qed
+   qed
+ next
+   case 2
+   have "(\<nexists>u. Ex (undirected_multigraph.decycle_multi (t_set (vset_insert e (id S))) u))"
+   proof(rule ccontr,goal_cases)
+     case 1
+     then obtain u C where uC:"undirected_multigraph.decycle_multi (insert e (t_set S)) u C"
+       using case_assms(1) dfs.Graph.vset.set.set_insert by fastforce
+     hence C_prop: "epath (to_dbltn ` insert e (t_set S)) u (map to_dbltn C) u"
+                    "set C \<subseteq> insert e (t_set S)" " 2 \<le> length C" "distinct C"
+       using uC[simplified undirected_multigraph.decycle_multi_def] by auto
+     have e_in_C:"e \<in> set C"
+     proof(rule ccontr, goal_cases)
+       case 1
+       hence "undirected_multigraph.decycle_multi (t_set S) u C"
+         using uC epath_subset_other_set[of "(to_dbltn ` insert e (t_set S))" 
+                    u "map to_dbltn C" u "to_dbltn ` (t_set S)"] 
+         by (simp add: image_mono subset_insert undirected_multigraph.decycle_multi_def)
+       then show ?case 
+         using assms(2)  case_assms(2) by(force simp add: undirected_multigraph.has_no_cycle_multi_def)
+     qed
+     obtain C1 C2 where C1C2:"C = C1@[e]@C2"
+       by (metis append_Cons append_Nil e_in_C in_set_conv_decomp_first)
+     hence epath_extended:"epath  (to_dbltn ` insert e (t_set S)) u (map to_dbltn (C1@[e]@C2@C1@[e]@C2@C1@[e]@C2)) u"
+       using epath_append C_prop(1)[simplified C1C2] by fastforce
+     have middle_three_rewrite:"xs@[x,y,z]@ys = (xs@[x])@[y]@(z#ys)" for x y z xs ys by auto
+     have e_path_very_verbose: "epath (to_dbltn ` insert e (t_set S)) u
+ (butlast (map to_dbltn (C1 @ [e] @ C2 @ C1)) @
+  [last (map to_dbltn (C1 @ [e] @ C2 @ C1)), to_dbltn e, hd (map to_dbltn (C2 @ C1 @ [e] @ C2))] @
+  tl (map to_dbltn (C2 @ C1 @ [e] @ C2))) u"
+       using epath_extended
+       apply(rule back_subst[of "\<lambda> p. epath _ _ p _ "])
+       apply(subst middle_three_rewrite) 
+       apply(subst append_butlast_last_id, simp)
+       apply(subst hd_Cons_tl,simp)
+       by auto
+     have "\<exists>x y. to_dbltn e = {x, y} \<and>
+      x \<noteq> y \<and>
+      epath (to_dbltn ` insert e (t_set S)) u
+       (butlast (map to_dbltn (C1 @ [e] @ C2 @ C1)) @ [last (map to_dbltn (C1 @ [e] @ C2 @ C1))]) x \<and>
+      epath (to_dbltn ` insert e (t_set S)) y
+       ([hd (map to_dbltn (C2 @ C1 @ [e] @ C2))] @ tl (map to_dbltn (C2 @ C1 @ [e] @ C2))) u \<and>
+      x \<in> last (map to_dbltn (C1 @ [e] @ C2 @ C1)) \<inter> to_dbltn e \<and>
+      y \<in> to_dbltn e \<inter> hd (map to_dbltn (C2 @ C1 @ [e] @ C2))"
+       using epath_find_splitter_advanced[OF e_path_very_verbose] by simp
+     then obtain x y where xy_prop:"to_dbltn e = {x, y}"
+      "x \<noteq> y"
+      "epath (to_dbltn ` insert e (t_set S)) u (map to_dbltn (C1 @ [e] @ C2 @ C1)) x"
+      "epath (to_dbltn ` insert e (t_set S)) y (map to_dbltn (C2 @ C1 @ [e] @ C2)) u"
+      "x \<in> last (map to_dbltn (C1 @ [e] @ C2 @ C1)) \<inter> to_dbltn e"
+      "y \<in> to_dbltn e \<inter> hd (map to_dbltn (C2 @ C1 @ [e] @ C2))" 
+       by(subst (asm) append_butlast_last_id, simp) force
+     have C1C2_empt:"C2@C1 \<noteq> []" 
+       using C1C2 C_prop(3) by force
+     define d1 where "d1 = last (C1 @ [e] @ C2 @ C1)"
+     have d1_def': "d1 = last (C2@C1)"
+       using C1C2_empt d1_def by auto
+     define d2 where "d2 = hd  (C2 @ C1 @ [e] @ C2)"
+     have d2_def': "d2 = hd (C2@C1)" 
+       using C1C2_empt  by(auto simp add: d2_def hd_append)
+     have xy_prop':"x \<in> to_dbltn d1 \<inter> to_dbltn e"
+                   "y \<in> to_dbltn e \<inter> to_dbltn d2" 
+       using xy_prop(5,6)
+       by(all \<open>subst (asm) last_map, simp\<close>, all \<open>subst (asm) hd_map, simp\<close>)
+          (auto simp add: d2_def d1_def)
+     have last_in:"d1 \<in> set C"
+       using C1C2   by(subst d1_def, intro set_rev_mp[OF last_in_set,of _  "set C"]) auto
+     have hd_in:"d2 \<in> set C"
+       using C1C2   by(subst d2_def, intro set_rev_mp[OF hd_in_set,of _  "set C"]) auto
+     have  d1_prop:"d1 \<in> set C" "to_dbltn e \<inter> to_dbltn d1 \<noteq> {}" 
+       using last_in xy_prop(1,5) by(all \<open>subst (asm) last_map, simp\<close>)(auto simp add: d1_def)
+     have  d2_prop:"d2 \<in> set C" "to_dbltn e \<inter> to_dbltn d2 \<noteq> {}" 
+       using hd_in xy_prop(1,6) by(all \<open>subst (asm) hd_map, simp\<close>)(auto simp add: d2_def)
+     have "d1 \<in> insert e (t_set S)" 
+       using C_prop(2) last_in by blast
+     moreover  have d1_not_e:"d1 \<noteq> e"
+     proof(rule ccontr, goal_cases)
+       case 1
+       hence "e \<in> set (C2@C1)"
+         using C1C2_empt d1_def' last_in_set by blast
+       hence "\<not> distinct C"
+         using C1C2 by fastforce
+       then show ?case
+         by (simp add: C_prop(4))
+     qed
+     ultimately have d1_in_S:"d1 \<in>  (t_set S)" 
+       by simp
+     have  "d2 \<in> insert e (t_set S)" 
+       using C_prop(2) hd_in by blast
+     moreover have d2_not_e:"d2 \<noteq> e"
+     proof(rule ccontr, goal_cases)
+       case 1
+       hence "e \<in> set (C2@C1)"
+         using C1C2_empt d2_def' hd_in_set by blast
+       hence "\<not> distinct C"
+         using C1C2 by fastforce
+       then show ?case
+         by (simp add: C_prop(4))
+     qed
+     ultimately have d2_in_S: "d2 \<in> (t_set S)" by simp
+
+     have dir_ds_in:"(v1_of d1, v2_of d1) \<in> G.digraph_abs (local.Kruskal_E_to_G S)"
+          "(v2_of d1, v1_of d1) \<in> G.digraph_abs (local.Kruskal_E_to_G S)"
+          "(v1_of d2, v2_of d2) \<in> G.digraph_abs (local.Kruskal_E_to_G S)"
+          "(v2_of d2, v1_of d2) \<in> G.digraph_abs (local.Kruskal_E_to_G S)"
+       by (simp add: d1_in_S d2_in_S digraph_abs_is)+
+     have graph_inv:"G.graph_inv (local.Kruskal_E_to_G S)" 
+       using local.Kruskal_E_to_G_def pair_graph_u_invar by force
+     have "lookup (local.Kruskal_E_to_G S) (v1_of e) \<noteq> None" 
+       using dir_ds_in  d1_prop(2) d2_prop(2) 2 d1_not_e d2_not_e  C1C2_empt  isin.simps(1)  xy_prop(1) xy_prop' 
+       apply(cases "lookup (local.Kruskal_E_to_G S) (v1_of d1)")
+       apply(all \<open>cases "lookup (local.Kruskal_E_to_G S) (v2_of d1)"\<close>)
+       apply(all \<open>cases "lookup (local.Kruskal_E_to_G S) (v1_of d2)"\<close>)
+       apply(all \<open>cases "lookup (local.Kruskal_E_to_G S) (v2_of d2)"\<close>)
+       apply(simp add: doubleton_eq_iff  G.neighbourhood_def Pair_Graph_RBT.G.are_connected_abs[OF graph_inv, symmetric])+
+       by metis
+     moreover have "lookup (local.Kruskal_E_to_G S) (v2_of e) \<noteq> None"
+       using dir_ds_in  d1_prop(2) d2_prop(2) 2 d1_not_e d2_not_e  C1C2_empt  isin.simps(1)  xy_prop(1) xy_prop' 
+       apply(cases "lookup (local.Kruskal_E_to_G S) (v1_of d1)")
+       apply(all \<open>cases "lookup (local.Kruskal_E_to_G S) (v2_of d1)"\<close>)
+       apply(all \<open>cases "lookup (local.Kruskal_E_to_G S) (v1_of d2)"\<close>)
+       apply(all \<open>cases "lookup (local.Kruskal_E_to_G S) (v2_of d2)"\<close>)
+       apply(simp add: doubleton_eq_iff  G.neighbourhood_def Pair_Graph_RBT.G.are_connected_abs[OF graph_inv, symmetric])+
+       by metis+
+     ultimately show ?case
+       using "2" by auto
+   qed
+   thus ?case 
+     using "2" by blast
+ qed
+qed
+  show ?case 
+    using second_eq dfs.Graph.vset.set.set_insert[OF assms(1)]
+    by (cases "rbt_subseteq (vset_insert e S) input_G ", 
+       unfold local_indep_oracle_def undirected_multigraph_spec.has_no_cycle_multi_def first_eq ) 
+       auto
+qed
+
+context fixes c::"'e \<Rightarrow> rat" and  order::"'e list"
+  assumes non_negative_c:"\<And> e. e \<in> t_set input_G \<Longrightarrow> c e \<ge> 0"
+and order_is_G: "t_set input_G = set order"
+and order_length_is_G_card: "distinct order"
+begin
+
+lemma best_in_greedy_axioms:"Best_In_Greedy.BestInGreedy_axioms vset_inv t_set set_of_sets_isin input_G
+     (Kruskal_Greedy2.indep_graph_matroid v1_of v2_of input_G)"
+    by(auto simp add:  Matroid_Specs_Inst.invar_def local.indep_graph_matroid_def set_of_sets_isin_def
+      Best_In_Greedy.BestInGreedy_axioms_def[OF Kruskal_Greedy2.Kruskal_Greedy.Best_In_Greedy_axioms] G_good Kruskal_Greedy2.indep_graph_matroid_def Matroid_Specs_Inst.indep_def
+      Matroid_Specs_Inst.finite_setsI)
+
+lemma sort_desc_axioms: "Best_In_Greedy.sort_desc_axioms Kruskal_Greedy.carrier_sorted"
+  by (simp add: Kruskal_Greedy.sort_desc_axioms_def insort_key_desc_stable
+ length_insort_key_desc set_insort_key_desc sorted_desc_f_insort_key_desc)
+
+lemma indep_system_axioms:"Matroid_Specs_Inst.indep_system_axioms input_G
+             (Kruskal_Greedy2.indep_graph_matroid v1_of v2_of input_G)"
+  unfolding  Matroid_Specs_Inst.indep_system_axioms_def
+proof(rule conjI[OF _ conjI], goal_cases)
+  case 1
+  then show ?case 
+  by(simp add: rbt_subseteq_correct[OF _ G_good, symmetric]
+           Matroid_Specs_Inst.indep_def Kruskal_Greedy2.indep_graph_matroid_def
+             indep_graph_matroid_def undirected_multigraph.has_no_cycle_multi_def
+             set_of_sets_isin_def) 
+next
+  case 2
+  show ?case
+    using undirected_multigraph.empty_has_no_cycle_multi_indep 
+    by(auto intro!: exI[of _ Leaf] 
+         simp add: Kruskal_Greedy.wrapper_axioms(5) Matroid_Specs_Inst.indep_def 
+                   Kruskal_Greedy2.indep_graph_matroid_def indep_graph_matroid_def set_of_sets_isin_def
+                    local.undirected_multigraph.empty_has_no_cycle_multi_indep)
+next
+  case 3
+  show ?case
+    unfolding Matroid_Specs_Inst.indep_def Kruskal_Greedy2.indep_graph_matroid_def indep_graph_matroid_def
+              set_of_sets_isin_def
+  proof(rule+, goal_cases)
+    case (1 X Y)
+    show ?case 
+      using 1(1,2,4) Custom_Set_RBT.set_subseteq 
+      by (auto intro:  undirected_multigraph.has_no_cycle_multi_indep_subset[OF 1(3)])
+  qed
+qed
+
+lemma nonnegative:" Kruskal_Greedy.nonnegative input_G c"
+  by(auto simp add: Kruskal_Greedy.nonnegative_def Pair_Graph_RBT.set.set_isin G_good  non_negative_c )
+
+lemma size_G_length_order:"size input_G = length order"
+  by(simp add:  G_good  Kruskal_Greedy2.rbt_size_correct distinct_card order_is_G order_length_is_G_card)
+
+lemma valid_order: "Kruskal_Greedy.valid_order input_G order"
+  by(simp add: Kruskal_Greedy.valid_order_def Pair_Graph_RBT.set.set_isin G_good  non_negative_c 
+                  size_G_length_order order_is_G)
+
+lemma kruskal_impl_corespondence: 
+  "to_ordinary (kruskal' v1_of v2_of input_G (kruskal_init' c order)) =
+  kruskal v1_of v2_of input_G (kruskal_init c order)"
+proof(rule Kruskal_Greedy.BestInGreedy'_corresp, goal_cases)
+  case (1 S x)
+  then show ?case 
+    by(unfold Kruskal_Greedy2.local_indep_oracle_def, intro local_indep_oracle_correct) auto
+next
+  case 2
+  then show ?case 
+    by (simp add: G_good)
+next
+  case 3
+  then show ?case
+    by (simp add: best_in_greedy_axioms) 
+next
+  case 4
+  then show ?case 
+    by (simp add: sort_desc_axioms)
+next
+  case 5
+  then show ?case
+    by (simp add: indep_system_axioms)
+next
+  case 6
+  then show ?case
+    by (simp add: nonnegative)
+next
+  case 7
+  then show ?case
+    by (simp add: valid_order)
+qed
+
+lemma indep_finite: "undirected_multigraph_spec.has_no_cycle_multi to_dbltn (t_set input_G) X \<Longrightarrow> finite X"
+  using Spanning_Trees.undirected_multigraph.graph_indep_system_multi indep_system.indep_finite
+ undirected_multigraph.undirected_multigraph_axioms by fast
+
+lemma idnep_in_G:"undirected_multigraph_spec.has_no_cycle_multi to_dbltn (t_set input_G) X \<Longrightarrow>
+           x \<in> X \<Longrightarrow> x \<in> t_set input_G"
+  using local.undirected_multigraph.has_no_cycle_multi_indep_subset_carrier by auto
+
+lemma indep_system_order:"indep_system (set order) (undirected_multigraph_spec.has_no_cycle_multi to_dbltn (set order))"
+  using local.undirected_multigraph.graph_indep_system_multi[of input_G] order_is_G by auto
+
+interpretation use_greedy_thms_kruskal:
+Use_Greedy_Thms Leaf vset_insert vset_delete isin t_set vset_inv vset_union
+                               vset_inter vset_diff rbt_subseteq  size set_of_sets_isin 
+"undirected_multigraph_spec.has_no_cycle_multi (\<lambda> e. {v1_of e, v2_of e})(Tree2.set_tree input_G)"
+input_G c order Kruskal_Greedy.carrier_sorted
+  by(intro Use_Greedy_Thms.intro 
+                      undirected_multigraph.graph_indep_system_multi indep_finite idnep_in_G)
+    (auto intro!: Use_Greedy_Thms_axioms.intro
+       simp add: Matroid_Specs_Inst.Matroid_Specs_axioms[simplified Matroid_Specs_def]
+                       set_of_sets_isin_def' G_good non_negative_c order_is_G
+                      indep_system_order indep_finite undirected_multigraph_spec.has_no_cycle_multi_def
+                      order_length_is_G_card sort_desc_axioms)
+
+lemma kruskal_returns_basis: "indep_system.basis (t_set input_G) 
+(undirected_multigraph_spec.has_no_cycle_multi to_dbltn (t_set input_G))
+ (t_set (result (kruskal v1_of v2_of input_G (kruskal_init c order))))"
+  by(simp add:  kruskal_def Kruskal_Greedy2.indep_graph_matroid_def local.indep_graph_matroid_def 
+                kruskal_init_def use_greedy_thms_kruskal.algo_gives_basis )
+
+corollary kruskal_returns_spanning_forest: 
+"undirected_multigraph_spec.is_spanning_forest_multi to_dbltn (t_set input_G)
+ (t_set (result (kruskal v1_of v2_of input_G (kruskal_init c order))))"
+  apply(subst undirected_multigraph.spanning_forest_iff_basis_multi)
+  by(rule kruskal_returns_basis)
+
+lemma rank_quotient_one: "indep_system.rank_quotient (t_set input_G)
+    (undirected_multigraph_spec.has_no_cycle_multi to_dbltn (t_set input_G)) = 1"
+  apply(subst Matroids_Theory.indep_system.matroid_iff_rq_eq_1[symmetric])
+  by (auto simp add: use_greedy_thms_kruskal.indep_system 
+                undirected_multigraph.graph_matroid_multi)
+
+theorem kruskal_is_max:
+"undirected_multigraph_spec.has_no_cycle_multi to_dbltn (t_set input_G) X \<Longrightarrow>
+sum c X \<le> sum c (t_set (result (kruskal v1_of v2_of input_G (kruskal_init c order))))"
+  unfolding kruskal_def kruskal_init_def Kruskal_Greedy2.indep_graph_matroid_def
+            local.indep_graph_matroid_def
+  apply(rule order.trans[rotated])
+  apply(rule use_greedy_thms_kruskal.indep_predicate_greedy_correct[of X])
+  by(simp add:  rank_quotient_one)+
+
+definition "max_forest X =
+ (undirected_multigraph_spec.is_spanning_forest_multi to_dbltn (t_set input_G) X
+\<and> (\<forall> Y. undirected_multigraph_spec.is_spanning_forest_multi to_dbltn (t_set input_G) Y \<longrightarrow>
+     sum c Y \<le> sum c X))"
+
+corollary kruskal_computes_max_spanning_forest:
+"max_forest(t_set (result (kruskal v1_of v2_of input_G (kruskal_init c order))))"
+  using kruskal_is_max kruskal_returns_spanning_forest 
+  by(auto simp add: max_forest_def undirected_multigraph.is_spanning_forest_multi_def)
+end
+end
+end
+
+
+definition "v1_of (e::(nat\<times>nat)) = min (fst e) (snd e)"
+definition "v2_of e = (if fst e = snd e then fst e + 1 else  max (fst e) (snd e))"
+
+interpretation kruskal_proof_maitroid_edges: Kruskal_Proof_Matroid_Edges v2_of G v1_of for G
+proof(rule  Kruskal_Proof_Matroid_Edges.intro, unfold v1_of_def v2_of_def, goal_cases)
+  case (1 e)
+  then show ?case 
+    by(cases "fst e = snd e") auto
+qed
+
+
+definition "edges = [(0::nat, 1::nat), (0, 2), (2, 3), (2,4), (2,1), (1,5), (5,8), (8,7), (7,1),
+                     (7,2), (7,4), (4,3), (3,4), (3,3), (9, 8), (8, 1), (4,5), (5,10)]"
+
+definition "G = foldr (\<lambda> x tree. vset_insert x  tree) edges empty"
+
+definition "c_list = [((0::nat, 1::nat), 1::rat), ((0, 2), 0.5), ((2, 3), 5/8), ((2,4), 3), ((2,1), -1/3),
+                      ((1,5), 4), ((5,8), 2), ((8,7), 0.1), ((7,1), 1.3),
+                     ((7,2), 3), ((7,4), 3), ((4,3), 2), ((3,4), 1), ((3,3), 0), ((9, 8),2.5),
+                      ((8, 1), 0), ((4,5), 2), ((5,10), 3)]"
+
+definition "c_impl = foldr (\<lambda> xy tree. update (prod.fst xy) (prod.snd xy) tree) c_list Leaf"
+value "c_impl"
+
+definition "costs  e =  (case (lookup c_impl e) of Some c \<Rightarrow> c | None \<Rightarrow> 0)"
+
+value "kruskal_init' costs edges"
+value  "kruskal' v1_of v2_of G (kruskal_init' costs edges)"
+value "inorder (result (kruskal' v1_of v2_of G (kruskal_init' costs edges)))"
+
+thm kruskal_proof_maitroid_edges.kruskal_computes_max_spanning_forest
+end
